derived the OCPL like statement as in the paper (+ malloc for adversary), use it for the read only example

theories/examples/lse_adequacy.v
@@ -7,12 +7,12 @@ From cap_machine Require Import
      rules logrel fundamental.
 From cap_machine.examples Require Import addr_reg_sample malloc macros_new lse.
 From cap_machine.examples Require Export mkregion_helpers disjoint_regions_tactics.
-From cap_machine.examples Require Import template_adequacy.
+From cap_machine.examples Require Import template_adequacy template_adequacy_ocpl.
 
 Instance DisjointList_list_Addr : DisjointList (list Addr).
 Proof. exact (@disjoint_list_default _ _ app []). Defined.
 
-Import with_adv_and_link.
+Import ocpl.
 
 Class memory_layout `{MachineParameters} := {
   (* Code of f *)
@@ -31,31 +31,31 @@ Class memory_layout `{MachineParameters} := {
   adv_region_start_offset: (adv_region_start + 1)%a = Some adv_start;
 
   (* malloc routine *)
-  malloc_start : Addr;
-  malloc_memptr : Addr;
-  malloc_mem_start : Addr;
-  malloc_end : Addr;
+  l_malloc_start : Addr;
+  l_malloc_memptr : Addr;
+  l_malloc_mem_start : Addr;
+  l_malloc_end : Addr;
 
-  malloc_code_size :
-    (malloc_start + length malloc_subroutine_instrs)%a
-    = Some malloc_memptr;
+  l_malloc_code_size :
+    (l_malloc_start + length malloc_subroutine_instrs)%a
+    = Some l_malloc_memptr;
 
-  malloc_memptr_size :
-    (malloc_memptr + 1)%a = Some malloc_mem_start;
+  l_malloc_memptr_size :
+    (l_malloc_memptr + 1)%a = Some l_malloc_mem_start;
 
-  malloc_mem_size :
-    (malloc_mem_start <= malloc_end)%a;
+  l_malloc_mem_size :
+    (l_malloc_mem_start <= l_malloc_end)%a;
 
   (* fail routine *)
-  fail_start : Addr;
-  fail_end : Addr;
+  l_fail_start : Addr;
+  l_fail_end : Addr;
 
-  fail_size :
-    (fail_start
+  l_fail_size :
+    (l_fail_start
      + (length assert_fail_instrs (* code of the subroutine *)
         + 1 (* pointer to the flag *))
     )%a
-    = Some fail_end;
+    = Some l_fail_end;
 
   (* link table *)
   link_table_start : Addr;
@@ -71,23 +71,23 @@ Class memory_layout `{MachineParameters} := {
     (adv_link_table_start + 1)%a = Some adv_link_table_end;
 
   (* failure flag *)
-  fail_flag : Addr;
-  fail_flag_next : Addr;
-  fail_flag_size :
-    (fail_flag + 1)%a = Some fail_flag_next;
+  l_fail_flag : Addr;
+  l_fail_flag_next : Addr;
+  l_fail_flag_size :
+    (l_fail_flag + 1)%a = Some l_fail_flag_next;
 
   (* disjointness of all the regions above *)
   regions_disjoint :
     ## [
         region_addrs adv_region_start adv_end;
         region_addrs f_region_start f_end;
-        [fail_flag];
+        [l_fail_flag];
         region_addrs link_table_start link_table_end;
         region_addrs adv_link_table_start adv_link_table_end;
-        region_addrs fail_start fail_end;
-        region_addrs malloc_mem_start malloc_end;
-        [malloc_memptr];
-        region_addrs malloc_start malloc_memptr
+        region_addrs l_fail_start l_fail_end;
+        region_addrs l_malloc_mem_start l_malloc_end;
+        [l_malloc_memptr];
+        region_addrs l_malloc_start l_malloc_memptr
        ]
 }.
 
@@ -103,40 +103,41 @@ Definition adv_prog `{memory_layout} : prog :=
      prog_instrs := adv_instrs ;
      prog_size := adv_size |}.
 
-(* MALLOC library entry *)
-Definition malloc_library_content `{memory_layout} : gmap Addr Word :=
-  (* code for the malloc subroutine *)
-  mkregion malloc_start malloc_memptr malloc_subroutine_instrs
-  (* Capability to malloc's memory pool, used by the malloc subroutine *)
-  ∪ list_to_map [(malloc_memptr, WCap RWX malloc_memptr malloc_end malloc_mem_start)]
-  (* Malloc's memory pool, initialized to zero *)
-  ∪ mkregion malloc_mem_start malloc_end (region_addrs_zeroes malloc_mem_start malloc_end).
+Program Definition layout `{memory_layout} : ocpl_library :=
+  {| (* malloc library *)
+     malloc_start := l_malloc_start;
+     malloc_memptr := l_malloc_memptr;
+     malloc_mem_start := l_malloc_mem_start;
+     malloc_end := l_malloc_end;
 
-Definition lib_entry_malloc `{memory_layout} : lib_entry :=
-  {| lib_start := malloc_start ;
-     lib_end := malloc_end ;
-     lib_entrypoint := malloc_start ;
-     lib_full_content := malloc_library_content |}.
+     malloc_code_size := l_malloc_code_size;
 
-(* FAIL library entry *)
-Definition fail_library_content `{memory_layout} : gmap Addr Word :=
-  (* code for the failure subroutine *)
-  (* tail contains pointer to the "failure" flag, set to 1 by the routine *)
-  mkregion fail_start fail_end (assert_fail_instrs ++ [WCap RW fail_flag fail_flag_next fail_flag])
-  ∪ list_to_map [(fail_flag, WInt 0%Z)] (* failure flag, initially set to 0 *).
+     malloc_memptr_size := l_malloc_memptr_size;
 
-Definition lib_entry_fail `{memory_layout} : lib_entry :=
-  {| lib_start := fail_start ;
-     lib_end := fail_end ;
-     lib_entrypoint := fail_start ;
-     lib_full_content := fail_library_content |}.
+     malloc_mem_size := l_malloc_mem_size;
 
-(* full library *)
-Definition library `{memory_layout} : lib :=
-  {| priv_libs := [lib_entry_fail] ;
-     pub_libs := [lib_entry_malloc] |}.
+     (* assertion fail library *)
+     fail_start := l_fail_start;
+     fail_end := l_fail_end;
 
-Program Definition roe_table `{memory_layout} : @tbl_priv roe_prog library :=
+     fail_size := l_fail_size;
+
+     fail_flag := l_fail_flag;
+     fail_flag_next := l_fail_flag_next;
+     fail_flag_size := l_fail_flag_size;
+
+     (* disjointness of the two libraries *)
+     libs_disjoint := _
+  |}.
+Next Obligation.
+  intros.
+  pose proof (regions_disjoint) as Hdisjoint.
+  rewrite !disjoint_list_cons in Hdisjoint |- *. intros (?&?&?&?&?&?&?&?&?).
+  set_solver.
+Qed.
+Definition OCPLLibrary `{memory_layout} := library layout.
+
+Program Definition roe_table `{memory_layout} : @tbl_priv roe_prog OCPLLibrary :=
   {| prog_lower_bound := f_region_start ;
      tbl_start := link_table_start ;
      tbl_end := link_table_end ;
@@ -151,7 +152,7 @@ Next Obligation.
   disjoint_map_to_list. set_solver.
 Qed.
 
-Program Definition adv_table `{memory_layout} : @tbl_pub adv_prog library :=
+Program Definition adv_table `{memory_layout} : @tbl_pub adv_prog OCPLLibrary :=
   {| prog_lower_bound := adv_region_start ;
      tbl_start := adv_link_table_start ;
      tbl_end := adv_link_table_end ;
@@ -166,87 +167,19 @@ Next Obligation.
   disjoint_map_to_list. set_solver.
 Qed.
 
-
-Definition OK_invariant `{MachineParameters} `{memory_layout} (m : gmap Addr Word) : Prop :=
-  ∀ w, m !! fail_flag = Some w → w = WInt 0%Z.
-
-Definition OK_dom `{MachineParameters} `{memory_layout} : gset Addr := {[ fail_flag ]}.
-
-Program Definition OK_dom_correct `{MachineParameters} `{memory_layout} :
-  ∀ m m',
-    (∀ a, a ∈ OK_dom → ∃ x, m !! a = Some x ∧ m' !! a = Some x) →
-    OK_invariant m ↔ OK_invariant m'.
-Proof.
-  intros m m' Hdom.
-  destruct Hdom with fail_flag as [w [Hw1 Hw2] ]. set_solver.
-  split;intros HOK;intros w' Hw';simplify_eq;apply HOK;auto.
-Defined.
-
-Definition flag_inv `{MachineParameters} `{memory_layout} : memory_inv :=
-  {| minv := OK_invariant ;
-     minv_dom := {[ fail_flag ]} ;
-     minv_dom_correct := OK_dom_correct |}.
-
-Lemma flag_inv_is_initial_memory `{memory_layout} m :
-  is_initial_memory roe_prog adv_prog library roe_table adv_table m →
-  minv flag_inv m.
-Proof.
-  intros Hinit. intros a Hin.
-  destruct Hinit as (?&?&Hlibs&?&?&?&Hlibdisj).
-  cbn in Hlibs. rewrite map_union_empty in Hlibs.
-  assert (fail_library_content ⊆ m) as Hfail.
-  { etrans;[|eauto]. apply map_union_subseteq_r. cbn in Hlibdisj.
-    rewrite !map_union_empty in Hlibdisj. auto. }
-  rewrite /fail_library_content in Hfail.
-  assert (list_to_map [(fail_flag, WInt 0)] ⊆ m) as Hfail_flag.
-  { etrans;[|eauto]. apply map_union_subseteq_r. disjoint_map_to_list.
-    pose proof (regions_disjoint) as Hdisjoint.
-    rewrite !disjoint_list_cons in Hdisjoint |- *. intros (?&?&?&?&?&?&?&?&?).
-    set_solver. }
-  simpl in Hfail_flag.
-  eapply (lookup_weaken _ _ fail_flag (WInt 0)) in Hfail_flag.
-  by simplify_eq. by simplify_map_eq.
-Qed.
-
-Lemma flag_inv_sub `{memory_layout} :
-  minv_dom flag_inv ⊆ dom (gset Addr) (lib_region (priv_libs library)).
-Proof.
-  cbn. rewrite map_union_empty.
-  intros Hinit. rewrite /fail_library_content.
-  rewrite /= dom_union_L dom_insert_L dom_empty_L.
-  rewrite union_empty_r. apply union_subseteq_r.
-Qed.
-
-(* TODO: move to iris extra *)
-Lemma big_sepM_to_big_sepL2 (PROP : bi) (A B : Type) `{EqDecision A} `{Countable A}
-      (φ: A -> B -> PROP) (l1: list A) (l2: list B):
-      NoDup l1 -> length l1 = length l2 →
-      ⊢ (([∗ map] y1↦y2 ∈ list_to_map (zip l1 l2), φ y1 y2) -∗
-         ([∗ list] y1;y2 ∈ l1;l2, φ y1 y2))%I.
-Proof.
-  revert l2. iInduction (l1) as [|x l1] "IH"; iIntros (l2 Hnd Hlen) "H".
-  - iSimpl. destruct l2;inversion Hlen. done.
-  - destruct l2;inversion Hlen. simpl.
-    inversion Hnd. subst.
-    iDestruct (big_sepM_insert with "H") as "[A B]".
-    + eapply not_elem_of_list_to_map.
-      rewrite fst_zip; auto. lia.
-    + iFrame. iApply ("IH" $! l2 H4 H1 with "B"); auto.
-Qed.
-
 Section roe_adequacy.
   Context {Σ:gFunctors} {memg:memG Σ} {regg:regG Σ}
           {nainv: logrel_na_invs Σ}
           `{memlayout: memory_layout}.
 
-  Definition mallocN : namespace := nroot .@ "roe" .@ "malloc".
-
   Lemma roe_correct :
     Forall (λ w, is_cap w = false) adv_instrs →
-    let filtered_map := λ (m : gmap Addr Word), filter (fun '(a, _) => a ∉ minv_dom flag_inv) m in
+    let filtered_map := λ (m : gmap Addr Word), filter (fun '(a, _) => a ∉ minv_dom (flag_inv layout)) m in
   (∀ rmap,
       dom (gset RegName) rmap = all_registers_s ∖ {[ PC; r_adv ]} →
-      ⊢ inv invN (minv_sep flag_inv)
+      ⊢ inv invN (minv_sep (flag_inv layout))
+        ∗ na_inv logrel_nais mallocN (mallocInv layout)
+        ∗ na_inv logrel_nais failflagN (assertInv layout)
         ∗ na_own logrel_nais ⊤
         ∗ PC ↦ᵣ WCap RWX (prog_lower_bound roe_table) (prog_end roe_prog) (prog_start roe_prog)
         ∗ r_adv ↦ᵣ WCap RWX (prog_lower_bound adv_table) (prog_end adv_prog) (prog_start adv_prog)
@@ -259,17 +192,14 @@ Section roe_adequacy.
         ∗ (prog_lower_bound adv_table) ↦ₐ (WCap RO (tbl_start adv_table) (tbl_end adv_table) (tbl_start adv_table))
         ∗ ([∗ map] a↦w ∈ (tbl_region adv_table), a ↦ₐ w)
         ∗ ([∗ map] a↦w ∈ (prog_region adv_prog), a ↦ₐ w)
-        (* filtered entries *)
-        ∗ ([∗ map] a↦w ∈ (lib_region (pub_libs library)), a ↦ₐ w)
-        ∗ ([∗ map] a↦w ∈ filtered_map (lib_region (priv_libs library)), a ↦ₐ w)
 
         -∗ WP Seq (Instr Executable) {{ λ _, True }}).
   Proof.
-    iIntros (Hints Hfilter rmap Hdom) "(#Hinv & Hown & HPC & Hr_adv & Hrmap & Hroe_link & Hroe_table & Hroe
-                                 & Hadv_link & Hadv_table & Hadv & Hpubs & Hprivs)".
+    iIntros (Hints Hfilter rmap Hdom) "(#Hinv & #Hmalloc & #Hassert & Hown & HPC & Hr_adv & Hrmap & Hroe_link & Hroe_table & Hroe
+                                 & Hadv_link & Hadv_table & Hadv)".
 
     iDestruct (big_sepM_sep with "Hrmap") as "[Hrmap #Hrmapvalid]".
-    simpl. rewrite !map_union_empty.
+    simpl.
 
     (* setting up read only example program *)
     iAssert (roe (region_addrs f_start f_end) 0 1 r_adv) with "[Hroe] "as "Hroe".
@@ -292,32 +222,8 @@ Section roe_adequacy.
     iDestruct (big_sepM_insert with "Hroe_table") as "[Hlink_table_mid _]";auto.
     iDestruct (big_sepM_insert with "Hadv_table") as "[Hadv_link_table_start _]";auto.
 
-    (* allocate malloc invariant *)
-    iMod (na_inv_alloc logrel_nais ⊤ mallocN (malloc_inv malloc_start malloc_end)
-            with "[Hpubs]") as "#Hinv_malloc".
-    { iNext. rewrite /malloc_inv. iExists malloc_memptr, malloc_mem_start.
-      rewrite /malloc_library_content.
-      iDestruct (big_sepM_union with "Hpubs") as "[Hpubs Hinit]".
-      { pose proof (regions_disjoint) as Hdisjoint.
-        rewrite !disjoint_list_cons in Hdisjoint |- *. intros (?&?&?&?&?&?&?&?&?).
-        disjoint_map_to_list. set_solver. }
-      iDestruct (big_sepM_union with "Hpubs") as "[Hpubs Hmid]".
-      { pose proof (regions_disjoint) as Hdisjoint.
-        rewrite !disjoint_list_cons in Hdisjoint |- *. intros (?&?&?&?&?&?&?&?&?).
-        disjoint_map_to_list. set_solver. }
-      pose proof malloc_code_size as Hmalloc_size.
-      pose proof malloc_memptr_size as Hmalloc_memptr_size.
-      pose proof malloc_mem_size as Hmalloc_mem_size.
-      iSplitL "Hpubs".
-      iApply big_sepM_to_big_sepL2. apply region_addrs_NoDup.
-      rewrite region_addrs_length /region_size.  solve_addr +Hmalloc_size.
-      assert ((malloc_start ^+ length malloc_subroutine_instrs)%a = malloc_memptr) as ->
-      ;[solve_addr+Hmalloc_size|iFrame].
-      iSplit;[auto|]. iDestruct (big_sepM_insert with "Hmid") as "[$ _]";auto.
-      iSplit;[|iPureIntro;solve_addr+Hmalloc_size Hmalloc_memptr_size Hmalloc_mem_size].
-      iApply big_sepM_to_big_sepL2. apply region_addrs_NoDup.
-      rewrite region_addrs_length replicate_length /region_size. solve_addr +Hmalloc_mem_size. iFrame. }
-    iDestruct (simple_malloc_subroutine_valid with "[$Hinv_malloc]") as "#Hmalloc_val".
+    (* determine malloc validity *)
+    iDestruct (simple_malloc_subroutine_valid with "[$Hmalloc]") as "#Hmalloc_val".
 
     (* allocate adversary table *)
     iMod (inv_alloc (logN .@ adv_link_table_start) ⊤ (interp_ref_inv adv_link_table_start interp)
@@ -349,7 +255,7 @@ Section roe_adequacy.
       iApply (big_sepL_mono with "Hadv'").
       iIntros (k y Hin) "Hint". iExists interp. iFrame. auto. }
 
-    iApply (roe_spec with "[- $HPC $Hown $Hr_adv $Hroe_link $Hrmap $Hroe $Hinv_malloc
+    iApply (roe_spec with "[- $HPC $Hown $Hr_adv $Hroe_link $Hrmap $Hroe $Hmalloc
                               $Hlink_table_start $Hlink_table_mid $Hadv_valid]");auto.
     instantiate (1:=f_end).
     { intros mid Hmid'. split;auto. pose proof (f_region_start_offset) as HH. solve_addr+HH Hmid'. }
@@ -361,11 +267,11 @@ Section roe_adequacy.
     iApply (inv_iff with "Hinv []"). iNext. iModIntro.
     iSplit.
     - rewrite /minv_sep /=. iIntros "HH". iDestruct "HH" as (m) "(Hm & %Heq & %HOK)".
-      assert (is_Some (m !! fail_flag)) as [? Hlook].
+      assert (is_Some (m !! l_fail_flag)) as [? Hlook].
       { apply elem_of_gmap_dom. rewrite Heq. apply elem_of_singleton. auto. }
-      iDestruct (big_sepM_lookup _ _ fail_flag with "Hm") as "Hflag";eauto.
+      iDestruct (big_sepM_lookup _ _ l_fail_flag with "Hm") as "Hflag";eauto.
       apply HOK in Hlook as ->. iFrame.
-    - iIntros "HH". iExists {[ fail_flag := WInt 0%Z ]}.
+    - iIntros "HH". iExists {[ l_fail_flag := WInt 0%Z ]}.
       rewrite big_sepM_singleton. iFrame.
       rewrite dom_singleton_L /minv_dom /=. iSplit;auto.
       rewrite /OK_invariant. iPureIntro. intros w Hw. simplify_map_eq. done.
@@ -375,18 +281,16 @@ End roe_adequacy.
 
 Theorem template_adequacy `{memory_layout}
     (m m': Mem) (reg reg': Reg) (es: list cap_lang.expr):
-  is_initial_memory roe_prog adv_prog library roe_table adv_table m →
-  is_initial_registers roe_prog adv_prog library roe_table adv_table reg r_adv →
+  is_initial_memory roe_prog adv_prog OCPLLibrary roe_table adv_table m →
+  is_initial_registers roe_prog adv_prog OCPLLibrary roe_table adv_table reg r_adv →
   Forall (λ w, is_cap w = false) (prog_instrs adv_prog) →
 
   rtc erased_step ([Seq (Instr Executable)], (reg, m)) (es, (reg', m')) →
-  (∀ w, m' !! fail_flag = Some w → w = WInt 0%Z).
+  (∀ w, m' !! l_fail_flag = Some w → w = WInt 0%Z).
 Proof.
   intros ? ? Hints ?.
   set (Σ' := #[]).
-  pose proof (template_adequacy Σ' roe_prog adv_prog library roe_table adv_table flag_inv) as Hadequacy.
+  pose proof (ocpl_template_adequacy Σ' layout roe_prog adv_prog roe_table adv_table) as Hadequacy.
   eapply Hadequacy;eauto.
-  { apply flag_inv_is_initial_memory. auto. }
-  { apply flag_inv_sub. }
   intros Σ ? ? ? ?. apply roe_correct. apply Hints.
 Qed.
