theories/examples/template_adequacy_ocpl.v
@@ -1,0 +1,280 @@
+From iris.algebra Require Import auth agree excl gmap gset frac.
+From iris.proofmode Require Import tactics.
+From iris.base_logic Require Import invariants.
+From iris.program_logic Require Import adequacy.
+From cap_machine Require Import
+     stdpp_extra iris_extra
+     rules logrel fundamental.
+From cap_machine.examples Require Import addr_reg_sample malloc macros_new.
+From cap_machine.examples Require Export mkregion_helpers disjoint_regions_tactics.
+From cap_machine.examples Require Import template_adequacy.
+
+Module ocpl.
+Include with_adv_and_link.
+
+Record ocpl_library `{MachineParameters} := MkOcplLibrary {
+  (* malloc library *)
+  malloc_start : Addr;
+  malloc_memptr : Addr;
+  malloc_mem_start : Addr;
+  malloc_end : Addr;
+
+  malloc_code_size :
+    (malloc_start + length malloc_subroutine_instrs)%a
+    = Some malloc_memptr;
+
+  malloc_memptr_size :
+    (malloc_memptr + 1)%a = Some malloc_mem_start;
+
+  malloc_mem_size :
+    (malloc_mem_start <= malloc_end)%a;
+
+  (* assertion fail library *)
+  fail_start : Addr;
+  fail_end : Addr;
+
+  fail_size :
+    (fail_start
+     + (length assert_fail_instrs (* code of the subroutine *)
+        + 1 (* pointer to the flag *))
+    )%a
+    = Some fail_end;
+
+  fail_flag : Addr;
+  fail_flag_next : Addr;
+  fail_flag_size :
+    (fail_flag + 1)%a = Some fail_flag_next;
+
+  (* disjointness of the two libraries *)
+  libs_disjoint :     ## [
+      [fail_flag];
+      region_addrs fail_start fail_end;
+      region_addrs malloc_mem_start malloc_end;
+      [malloc_memptr];
+      region_addrs malloc_start malloc_memptr
+     ]
+}.
+
+Definition malloc_library_content `{MachineParameters} (layout : ocpl_library) : gmap Addr Word :=
+  (* code for the malloc subroutine *)
+  mkregion (malloc_start layout) (malloc_memptr layout) malloc_subroutine_instrs
+  (* Capability to malloc's memory pool, used by the malloc subroutine *)
+  ∪ list_to_map [((malloc_memptr layout), WCap RWX (malloc_memptr layout) (malloc_end layout) (malloc_mem_start layout))]
+  (* Malloc's memory pool, initialized to zero *)
+  ∪ mkregion (malloc_mem_start layout) (malloc_end layout) (region_addrs_zeroes (malloc_mem_start layout) (malloc_end layout)).
+
+Definition lib_entry_malloc `{MachineParameters} (layout : ocpl_library) : lib_entry :=
+  {| lib_start := malloc_start layout;
+     lib_end := malloc_end layout;
+     lib_entrypoint := malloc_start layout;
+     lib_full_content := malloc_library_content layout|}.
+
+(* FAIL library entry *)
+Definition fail_library_content `{MachineParameters} (layout : ocpl_library) : gmap Addr Word :=
+  (* code for the failure subroutine *)
+  (* tail contains pointer to the "failure" flag, set to 1 by the routine *)
+  mkregion (fail_start layout) (fail_end layout) (assert_fail_instrs ++ [WCap RW (fail_flag layout) (fail_flag_next layout) (fail_flag layout)])
+  ∪ list_to_map [((fail_flag layout), WInt 0%Z)] (* failure flag, initially set to 0 *).
+
+Definition lib_entry_fail `{MachineParameters} (layout : ocpl_library) : lib_entry :=
+  {| lib_start := fail_start layout;
+     lib_end := fail_end layout;
+     lib_entrypoint := fail_start layout;
+     lib_full_content := fail_library_content layout |}.
+
+(* full library *)
+Definition library `{MachineParameters} (layout : ocpl_library) : lib :=
+  {| priv_libs := [lib_entry_fail layout] ;
+     pub_libs := [lib_entry_malloc layout] |}.
+
+Definition OK_invariant `{MachineParameters} (layout : ocpl_library) (m : gmap Addr Word) : Prop :=
+  ∀ w, m !! (fail_flag layout) = Some w → w = WInt 0%Z.
+
+Definition OK_dom `{MachineParameters} (layout : ocpl_library) : gset Addr := {[ fail_flag layout ]}.
+
+Program Definition OK_dom_correct `{MachineParameters} (layout : ocpl_library) :
+  ∀ m m',
+    (∀ a, a ∈ OK_dom layout → ∃ x, m !! a = Some x ∧ m' !! a = Some x) →
+    OK_invariant layout m ↔ OK_invariant layout m'.
+Proof.
+  intros m m' Hdom.
+  destruct Hdom with (fail_flag layout) as [w [Hw1 Hw2] ]. rewrite /OK_dom. set_solver.
+  split;intros HOK;intros w' Hw';simplify_eq;apply HOK;auto.
+Defined.
+
+Definition flag_inv `{MachineParameters} (layout : ocpl_library) : memory_inv :=
+  {| minv := OK_invariant layout;
+     minv_dom := {[ fail_flag layout ]} ;
+     minv_dom_correct := OK_dom_correct layout |}.
+
+Lemma flag_inv_is_initial_memory `{MachineParameters} (layout : ocpl_library) trusted_prog adv_prog trusted_table adv_table m :
+  is_initial_memory trusted_prog adv_prog (library layout) trusted_table adv_table m →
+  minv (flag_inv layout) m.
+Proof.
+  intros Hinit. intros a Hin.
+  destruct Hinit as (?&?&Hlibs&?&?&?&Hlibdisj).
+  cbn in Hlibs. rewrite map_union_empty in Hlibs.
+  assert ((fail_library_content layout) ⊆ m) as Hfail.
+  { etrans;[|eauto]. apply map_union_subseteq_r. cbn in Hlibdisj.
+    rewrite !map_union_empty in Hlibdisj. auto. }
+  rewrite /fail_library_content in Hfail.
+  assert (list_to_map [(fail_flag layout, WInt 0)] ⊆ m) as Hfail_flag.
+  { etrans;[|eauto]. apply map_union_subseteq_r. disjoint_map_to_list.
+    pose proof (libs_disjoint layout) as Hdisjoint.
+    rewrite !disjoint_list_cons in Hdisjoint |- *. intros (?&?&?&?&?&?).
+    set_solver. }
+  simpl in Hfail_flag.
+  eapply (lookup_weaken _ _ (fail_flag layout) (WInt 0)) in Hfail_flag.
+    by simplify_eq. by simplify_map_eq.
+Qed.
+
+Lemma flag_inv_sub `{MachineParameters} (layout : ocpl_library) :
+  minv_dom (flag_inv layout) ⊆ dom (gset Addr) (lib_region (priv_libs (library layout))).
+Proof.
+  cbn. rewrite map_union_empty.
+  intros Hinit. rewrite /fail_library_content.
+  rewrite /= dom_union_L dom_insert_L dom_empty_L.
+  rewrite union_empty_r. apply union_subseteq_r.
+Qed.
+
+(* TODO: move to iris extra *)
+Lemma big_sepM_to_big_sepL2 (PROP : bi) (A B : Type) `{EqDecision A} `{Countable A}
+      (φ: A -> B -> PROP) (l1: list A) (l2: list B):
+      NoDup l1 -> length l1 = length l2 →
+      ⊢ (([∗ map] y1↦y2 ∈ list_to_map (zip l1 l2), φ y1 y2) -∗
+         ([∗ list] y1;y2 ∈ l1;l2, φ y1 y2))%I.
+Proof.
+  revert l2. iInduction (l1) as [|x l1] "IH"; iIntros (l2 Hnd Hlen) "H".
+  - iSimpl. destruct l2;inversion Hlen. done.
+  - destruct l2;inversion Hlen. simpl.
+    inversion Hnd. subst.
+    iDestruct (big_sepM_insert with "H") as "[A B]".
+    + eapply not_elem_of_list_to_map.
+      rewrite fst_zip; auto. lia.
+    + iFrame. iApply ("IH" $! l2 H4 H1 with "B"); auto.
+Qed.
+Lemma map_filter_id :
+  ∀ (K : Type) (M : Type → Type) (H : FMap M) (H0 : ∀ A : Type, Lookup K A (M A)) (H1 : ∀ A : Type, Empty (M A)) (H2 : ∀ A : Type, PartialAlter K A (M A))
+    (H3 : OMap M) (H4 : Merge M) (H5 : ∀ A : Type, FinMapToList K A (M A)) (EqDecision0 : EqDecision K),
+    FinMap K M
+    → ∀ (A : Type) (P : K * A → Prop) (H7 : ∀ x : K * A, Decision (P x)) (m : M A),
+      (∀ i x, m !! i = Some x → P (i, x)) → filter P m = m.
+Proof.
+  intros. apply map_eq.
+  intros i. destruct (m !! i) eqn:Hsome.
+  - apply map_filter_lookup_Some_2;auto.
+  - apply map_filter_lookup_None_2;auto.
+Qed.
+
+
+
+Definition assertInv `{memG Σ, regG Σ, MachineParameters} (layout : ocpl_library) :=
+  [[ fail_start layout, fail_end layout]]↦ₐ[[ assert_fail_instrs ++ [WCap RW (fail_flag layout) (fail_flag_next layout) (fail_flag layout)] ]]%I.
+Definition mallocInv `{memG Σ, regG Σ, MachineParameters} (layout : ocpl_library) :=
+  malloc_inv (malloc_start layout) (malloc_end layout).
+
+Definition mallocN : namespace := nroot .@ "pub" .@ "malloc".
+Definition failflagN : namespace := nroot .@ "priv" .@ "flag".
+
+Theorem ocpl_template_adequacy `{MachineParameters} (Σ : gFunctors)
+    (layout: ocpl_library)
+    (P Adv: prog)
+    (P_tbl : @tbl_priv P (library layout))
+    (Adv_tbl : @tbl_pub Adv (library layout)) (r_adv : RegName)
+    (m m': Mem) (reg reg': Reg) (es: list cap_lang.expr):
+  is_initial_memory P Adv (library layout) P_tbl Adv_tbl m →
+  is_initial_registers P Adv (library layout) P_tbl Adv_tbl reg r_adv →
+  Forall (λ w, is_cap w = false) (prog_instrs Adv) →
+
+  let filtered_map := λ (m : gmap Addr Word), filter (fun '(a, _) => a ∉ minv_dom (flag_inv layout)) m in
+  (∀ `{memG Σ', regG Σ', logrel_na_invs Σ', subG Σ Σ'} rmap,
+      dom (gset RegName) rmap = all_registers_s ∖ {[ PC; r_adv ]} →
+      ⊢ inv invN (minv_sep (flag_inv layout))
+        ∗ na_inv logrel_nais mallocN (mallocInv layout)
+        ∗ na_inv logrel_nais failflagN (assertInv layout)
+        ∗ na_own logrel_nais ⊤
+        ∗ PC ↦ᵣ WCap RWX (prog_lower_bound P_tbl) (prog_end P) (prog_start P)
+        ∗ r_adv ↦ᵣ WCap RWX (prog_lower_bound Adv_tbl) (prog_end Adv) (prog_start Adv)
+        ∗ ([∗ map] r↦w ∈ rmap, r ↦ᵣ w ∗ ⌜is_cap w = false⌝)
+        (* P program and table *)
+        ∗ (prog_lower_bound P_tbl) ↦ₐ (WCap RO (tbl_start P_tbl) (tbl_end P_tbl) (tbl_start P_tbl))
+        ∗ ([∗ map] a↦w ∈ (tbl_region P_tbl), a ↦ₐ w)
+        ∗ ([∗ map] a↦w ∈ (prog_region P), a ↦ₐ w)
+        (* Adv program and table *)
+        ∗ (prog_lower_bound Adv_tbl) ↦ₐ (WCap RO (tbl_start Adv_tbl) (tbl_end Adv_tbl) (tbl_start Adv_tbl))
+        ∗ ([∗ map] a↦w ∈ (tbl_region Adv_tbl), a ↦ₐ w)
+        ∗ ([∗ map] a↦w ∈ (prog_region Adv), a ↦ₐ w)
+
+        -∗ WP Seq (Instr Executable) {{ λ _, True }}) →
+
+  rtc erased_step ([Seq (Instr Executable)], (reg, m)) (es, (reg', m')) →
+  minv (flag_inv layout) m'.
+Proof.
+  set (Σ' := #[invΣ; gen_heapΣ Addr Word; gen_heapΣ RegName Word;
+              na_invΣ; Σ]).
+  intros ? ? ? ? Hspec.
+  eapply (template_adequacy Σ');[eauto..|]; (* rewrite /invPreG. solve_inG. *)
+    try typeclasses eauto.
+  eapply flag_inv_is_initial_memory;eauto.
+  eapply flag_inv_sub;eauto.
+  intros. cbn.
+  rewrite !map_union_empty.
+  iIntros "(#Hflag & Hown & HPC & Hr_adv & Hrmap & Htbl & Htbl_r
+           & Hprog & Htbl_adv & Htbl_adv_r & Hprog_adv & Hmalloc & Hfail)".
+
+  (* allocate malloc invariant *)
+  iMod (na_inv_alloc logrel_nais ⊤ mallocN (mallocInv layout)
+          with "[Hmalloc]") as "#Hinv_malloc".
+  { iNext. rewrite /mallocInv /malloc_inv. iExists (malloc_memptr layout), (malloc_mem_start layout).
+    rewrite /malloc_library_content.
+    iDestruct (big_sepM_union with "Hmalloc") as "[Hpubs Hinit]".
+    { pose proof (libs_disjoint layout) as Hdisjoint.
+      rewrite !disjoint_list_cons in Hdisjoint |- *. intros (?&?&?&?&?&?).
+      disjoint_map_to_list. set_solver. }
+    iDestruct (big_sepM_union with "Hpubs") as "[Hpubs Hmid]".
+    { pose proof (libs_disjoint layout) as Hdisjoint.
+      rewrite !disjoint_list_cons in Hdisjoint |- *. intros (?&?&?&?&?&?).
+      disjoint_map_to_list. set_solver. }
+    pose proof (malloc_code_size layout) as Hmalloc_size.
+    pose proof (malloc_memptr_size layout) as Hmalloc_memptr_size.
+    pose proof (malloc_mem_size layout) as Hmalloc_mem_size.
+    iSplitL "Hpubs".
+    iApply big_sepM_to_big_sepL2. apply region_addrs_NoDup.
+    rewrite region_addrs_length /region_size.
+    solve_addr +Hmalloc_size.
+    assert (((malloc_start layout) ^+ length malloc_subroutine_instrs)%a = (malloc_memptr layout)) as ->
+    ;[solve_addr+Hmalloc_size|iFrame].
+    iSplit;[auto|]. iDestruct (big_sepM_insert with "Hmid") as "[$ _]";auto.
+    iSplit;[|iPureIntro;solve_addr+Hmalloc_size Hmalloc_memptr_size Hmalloc_mem_size].
+    iApply big_sepM_to_big_sepL2. apply region_addrs_NoDup.
+    rewrite region_addrs_length replicate_length /region_size. solve_addr +Hmalloc_mem_size. iFrame. }
+
+  (* allocate the flag invariant *)
+  iMod (na_inv_alloc logrel_nais ⊤ failflagN (assertInv layout)
+          with "[Hfail]") as "#Hinv_fail".
+  { iNext. rewrite /assertInv /fail_library_content.
+    rewrite -insert_union_r.
+    pose proof (fail_flag_size layout) as Hfail_flag_size.
+    pose proof (fail_size layout) as Hfail_size.
+    rewrite map_union_empty map_filter_insert_not'.
+    rewrite map_filter_id.
+    - by iApply mkregion_sepM_to_sepL2.
+    - intros i x Hx.
+      assert (i ∈ region_addrs (fail_start layout) (fail_end layout)) as Hin.
+      { eapply in_dom_mkregion. apply elem_of_gmap_dom. eauto. }
+      intros Hcontr%elem_of_singleton_1. subst.
+      pose proof (libs_disjoint layout) as Hdisjoint.
+      rewrite !disjoint_list_cons in Hdisjoint |- *. intros (?&?&?&?&?&?).
+      set_solver.
+    - simpl. intros Hcontr. apply Hcontr. apply elem_of_singleton. auto.
+    - intros y _. intros Hcontr. apply Hcontr. apply elem_of_singleton. auto.
+    - apply not_elem_of_dom.
+      intros Hdom%in_dom_mkregion.
+      pose proof (libs_disjoint layout) as Hdisjoint.
+      rewrite !disjoint_list_cons in Hdisjoint |- *. intros (?&?&?&?&?&?).
+      set_solver. }
+
+  iApply Hspec;[..|iFrame "∗ #"];auto. solve_inG.
+Qed.
+
+End ocpl.
